matching-logic/src/Experimental/Unification/Definitions.v
@@ -38,7 +38,7 @@ Section Definitions.
 
        insertUP P (t, u) ~ P ∪ {t ≐ u}
      *)
-    insertUP : T -> (WFPattern * WFPattern) -> T;
+    insertUP : T -> (TermPattern * TermPattern) -> T;
     (** Failed unification problem
 
        bottomUP ~ ⊥
@@ -50,31 +50,31 @@ Section Definitions.
        toPredicateUP P ~ ϕᴾ
      *)
 
-    toPredicateUP : T -> WFPattern;
+    toPredicateUP : T -> WFMFPattern;
     (** Substitution of a variable to a pattern in every pattern of
        a unification problem
 
        substituteAllUP x t P ~ P{x ↦ t}
      *)
 
-    substituteAllUP : evar -> WFPattern -> T -> T;
+    substituteAllUP : evar -> TermPattern -> T -> T;
     (** Creation of a singleton problem
 
        singletonUP t u ~ {t ≐ u}
      *)
 
-    singletonUP : WFPattern -> WFPattern -> T;
+    singletonUP : TermPattern -> TermPattern -> T;
 
     (**
        Converting a unification problem maps insertion to conjunction.
      *)
-    toPredicateInsertUP : forall Γ t x y, Γ ⊢wf toPredicateUP (insertUP t (x, y)) wf<---> ((x wf=ml y) wfand (toPredicateUP t));
+    toPredicateInsertUP : forall Γ t x y, Γ ⊢ toPredicateUP (insertUP t (x, y)) wf<---> ((x wf=ml y) wfand (toPredicateUP t));
 
     (**
        Converting a unification problem maps substitution of unification problems
        to substitution of patterns.
      *)
-    toPredicateSubstituteAllUP : forall Γ t e p, Γ ⊢wf toPredicateUP (substituteAllUP e p t) wf<---> (toPredicateUP t)^wf[[evar:e↦p]];
+    toPredicateSubstituteAllUP : forall Γ t e p, Γ ⊢ toPredicateUP (substituteAllUP e p t) wf<---> (toPredicateUP t)^wf[[evar:e↦p]];
 
     (**
        Inserting into a non-⊥ unification problem cannot result ⊥.
@@ -84,93 +84,361 @@ Section Definitions.
     (**
        Converting a singleton problem to a predicate pattern gives us an equality.
      *)
-    toPredicateSingletonUP : forall Γ t1 t2, Γ ⊢wf toPredicateUP (singletonUP t1 t2) wf<---> (t1 wf=ml t2)
+    toPredicateSingletonUP : forall Γ t1 t2, Γ ⊢ toPredicateUP (singletonUP t1 t2) wf<---> (t1 wf=ml t2)
   }.
 
-  #[refine] Instance optionSetUP `{H : ElemOf (WFPattern * WFPattern) T, H0 : Empty T, H1 : Singleton (WFPattern * WFPattern) T, H2 : Union T, H3 : Intersection T, H4 : Difference T, H5 : Elements (WFPattern * WFPattern) T, @FinSet (WFPattern * WFPattern) T H H0 H1 H2 H3 H4 H5 WFPattern_eq_dec, !LeibnizEquiv T} : UP (option T) := {
+  Local Definition wfmfTop := mkWFMF Top well_formed_top eq_refl.
+
+  Goal forall φ a b c, (a ≠ c) -> (patt_free_evar c)^[[evar:a↦patt_free_evar b]]^[[evar:c↦φ]] = φ.
+  Proof.
+    intros.
+    simpl.
+    rewrite decide_False. assumption.
+    simpl. rewrite decide_eq_same.
+    reflexivity.
+  Qed.
+
+  (* Lemma equality_elimination_functional_subst (Γ : Theory) p q p1 p2 x : *)
+  (*   theory ⊆ Γ -> *)
+  (*   well_formed p -> *)
+  (*   well_formed q -> *)
+  (*   well_formed p1 -> *)
+  (*   well_formed p2 -> *)
+  (*   mu_free p -> *)
+  (*   mu_free q -> *)
+  (*   pattern_kt_well_formed p1 -> *)
+  (*   pattern_kt_well_formed p2 -> *)
+  (*   Γ ⊢ p =ml q -> *)
+  (*   Γ ⊢ p1 =ml p2 -> *)
+  (*   Γ ⊢ is_functional p1 -> *)
+  (*   Γ ⊢ p^[[evar: x ↦ p1]] =ml q^[[evar: x ↦ p2]]. *)
+  (* Proof. *)
+  (*   intros HΓ Hwfp Hwfq Hwfp1 Hwfp2 Hmfp Hmfq Hktwfp1 Hktwfp2 Hpeqq Hp1eqp2 Hfuncp1. *)
+  (*   pose proof mf_imp_ktwf _ Hmfp as Hktwfp. *)
+  (*   pose proof mf_imp_ktwf _ Hmfq as Hktwfq. *)
+
+    (* apply universal_generalization with (x := x) in Hpeqq; *)
+    (* [| try_solve_pile | wf_auto2]. *)
+    (* eapply forall_functional_subst_meta with (φ' := p1) in Hpeqq; *)
+    (* auto; [|rewrite <- mu_free_evar_quantify | ..]; *)
+    (* [| wf_auto2 ..]. *)
+    (* rewrite bevar_subst_evar_quantify in Hpeqq; [wf_auto2 |]. *)
+    (* mlSimpl in Hpeqq. *)
+    (* mlFreshEvar as y. *)
+    (* unshelve epose proof MP Hp1eqp2 (equality_elimination Γ p1 p2 {|pcPattern := p^[[evar: x ↦ p1]] =ml q^[[evar: x ↦ patt_free_evar y]]; pcEvar := y|} HΓ _ _ _ _); try solve [wf_auto2]. *)
+    (* simpl. rewrite ! pattern_kt_well_formed_free_evar_subst; auto. *)
+    (* unfold emplace in H. mlSimpl in H. cbn in H. *)
+    (* rewrite -> 2 free_evar_subst_chain in H; [| fm_solve ..]. *)
+    (* rewrite -> 2 (free_evar_subst_no_occurrence y) in H; [| fm_solve ..]. *)
+    (* exact (MP Hpeqq H). *)
+  (* Defined. *)
+
+  (*Goal forall Γ p q p1 p2 x, *)
+  (*  theory ⊆ Γ -> *)
+  (*  well_formed p -> *)
+  (*  well_formed q -> *)
+  (*  well_formed p1 -> *)
+  (*  well_formed p2 -> *)
+  (*  mu_free p -> *)
+  (*  mu_free q -> *)
+  (*  pattern_kt_well_formed p1 -> *)
+  (*  pattern_kt_well_formed p2 -> *)
+  (*  Γ ⊢ p =ml q ---> *)
+  (*  p1 =ml p2 ---> *)
+  (*  is_functional p1 ---> *)
+  (*  p^[[evar: x ↦ p1]] =ml q^[[evar: x ↦ p2]]. *)
+  (*Proof. *)
+  (*  intros * HΓ Hwfp Hwfq Hwfp1 Hwfp2 Hmfp Hmfq Hktwfp1 Hktwfp2. *)
+  (*  pose proof mf_imp_ktwf _ Hmfp as Hktwfp. *)
+  (*  pose proof mf_imp_ktwf _ Hmfq as Hktwfq. *)
+  (*  toMLGoal. wf_auto2. do 3 mlIntro. *)
+  (*  mlFreshEvar as y. *)
+  (*  unshelve epose proof equality_elimination Γ p1 p2 {| pcEvar := y; pcPattern := p^[[evar:x↦p1]] =ml q^[[evar:x↦patt_free_evar y]] |} HΓ Hwfp1 Hwfp2 _ _. *)
+  (*  wf_auto2. *)
+  (*  simpl. rewrite ! pattern_kt_well_formed_free_evar_subst; auto. *)
+  (*  unfold emplace in H. cbn [pcPattern pcEvar] in H. *)
+  (*  mlSimpl in H. rewrite ! free_evar_subst_chain in H. *)
+  (*  ltac2:(fm_solve()). *)
+  (*  ltac2:(fm_solve()). *)
+  (*  rewrite ! (free_evar_subst_no_occurrence y) in H. *)
+  (*  ltac2:(fm_solve()). *)
+  (*  ltac2:(fm_solve()). *)
+  (*  mlApplyMeta H in "1". mlApply "1". clear H. mlClear "1". *)
+
+  (*  Search free_evar_subst. *)
+
+  (*  rewrite <- 2 bevar_subst_evar_quantify with (dbi := 0). *)
+  (*  2,3: wf_auto2. *)
+  (*  unshelve epose proof forall_functional_subst (p^{{evar:x↦0}} =ml q^{{evar:x↦0}}) p1 Γ HΓ _ Hwfp1 _ _. *)
+  (*  1-3: wf_auto2; rewrite <- mu_free_evar_quantify; auto. *)
+  (*  mlSimpl in H. mlApplyMeta H. clear H. *)
+  (*  mlSplitAnd. 2: mlExact "2". mlClear "2". *) 
+  (*  mlIntroAllManual y. *)
+  (*  fm_solve. *)
+  (*  simpl; rewrite ! free_evars_evar_quantify; fm_solve. *)
+  (*  try_solve_pile. *)
+    
+
+  (*  Search patt_forall. *)
+
+  (*  mlDeduct "0". *)
+  (*  remember (Γ ∪ _) as Γ'. *)
+  (*  remember (_ : ProofInfo) as i. *)
+  (*  unshelve epose proof universal_generalization Γ' (p =ml q) x i _ _. *)
+  (*  subst i. try_solve_pile. *)
+  (*  unfold pi_generalized_evars. rewrite ! union_empty_r_L. *)
+
+  (*  mlRevertAll x. *)
+  (*  epose proof universal_generalization Γ (p =ml q) x AnyReasoning (pile_any _) (well_formed_equal _ _ Hwfp Hwfq). *)
+  (*  mlApplyMeta H in "0". *)
+  (*  eapply forall_functional_subst_meta with (φ' := p1) in Hpeqq; *)
+  (*  auto; [|rewrite <- mu_free_evar_quantify | ..]; *)
+  (*  [| wf_auto2 ..]. *)
+  (*  rewrite bevar_subst_evar_quantify in Hpeqq; [wf_auto2 |]. *)
+  (*  mlSimpl in Hpeqq. *)
+  (*  mlFreshEvar as y. *)
+  (*  unshelve epose proof MP Hp1eqp2 (equality_elimination Γ p1 p2 {|pcPattern := p^[[evar: x ↦ p1]] =ml q^[[evar: x ↦ patt_free_evar y]]; pcEvar := y|} HΓ _ _ _ _); try solve [wf_auto2]. *)
+  (*  simpl. rewrite ! pattern_kt_well_formed_free_evar_subst; auto. *)
+  (*  unfold emplace in H. mlSimpl in H. cbn in H. *)
+  (*  rewrite -> 2 free_evar_subst_chain in H; [| fm_solve ..]. *)
+  (*  rewrite -> 2 (free_evar_subst_no_occurrence y) in H; [| fm_solve ..]. *)
+  (*  exact (MP Hpeqq H). *)
+  (*  Defined. *)
+
+    Goal forall Γ e a, theory ⊆ Γ -> e ≠ a -> {x & ((e ∈ free_evars x) * (Γ ⊢ x =ml patt_free_evar a))%type}.
+    Proof.
+      intros.
+      exists (patt_free_evar e and patt_bott or patt_free_evar a).
+      split.
+      set_solver.
+      toMLGoal. wf_auto2.
+      mlApplyMeta disj_equals_greater_1. 2: auto.
+      fromMLGoal.
+      apply phi_impl_total_phi_meta. wf_auto2. try_solve_pile.
+      mlIntro. mlDestructAnd "0". mlDestructBot "2".
+    Defined.
+
+    (* NOT TRUE *)
+    (* Goal forall x Γ e a, theory ⊆ Γ -> well_formed x -> e ∈ free_evars x -> e ≠ a -> Γ ⊢ ! x =ml patt_free_evar a. *)
+    (* Proof. *)
+    (*   induction x; intros. *)
+    (*   - simpl in H1. apply elem_of_singleton_1 in H1. *)
+    (*     rewrite <- H1. clear H1. *)
+    (*     mlIntro. *)
+    (*     (1* Search patt_equal. *1) *)
+    (*     unfold patt_equal, patt_total. *)
+    (*     mlApply "0". mlClear "0". *)
+    (*     unfold patt_iff. *)
+    (*     Search patt_not patt_and patt_or. *)
+    (*     unshelve epose proof deMorgan_nand Γ (patt_free_evar e ---> patt_free_evar a) (patt_free_evar a ---> patt_free_evar e) _ _. *)
+    (*     1-2: wf_auto2. use AnyReasoning in H1. *)
+    (*     mlRewrite H1 at 1. clear H1. *)
+    (*     mlApplyMeta patt_defined_or_2. *)
+    (*     2: assumption. *)
+    (*     unshelve epose proof and_impl_2 Γ (patt_free_evar e) (patt_free_evar a) _ _. 1-2: wf_auto2. *)
+    (*     use AnyReasoning in H1. mlRewrite H1 at 1. clear H1. *)
+    (*     unshelve epose proof and_impl_2 Γ (patt_free_evar a) (patt_free_evar e) _ _. 1-2: wf_auto2. *)
+    (*     use AnyReasoning in H1. mlRewrite H1 at 1. clear H1. *)
+    (*     Search patt_in. *)
+    (*     Search patt_defined. *)
+    (* Abort. *)
+
+    Goal forall (Γ : Theory) (φ ψ : Pattern) (e : evar), theory ⊆ Γ -> well_formed φ -> mu_free φ -> well_formed ψ -> e ∉ free_evars φ -> Γ ⊢ is_functional ψ ---> φ ---> φ^[[evar:e↦ψ]].
+    Proof.
+      intros.
+      epose proof universal_generalization_iter Γ [φ] φ e AnyReasoning ltac:(wf_auto2) H0 ltac:(unfold free_evars_of_list; set_solver) ltac:(try_solve_pile) (useBasicReasoning AnyReasoning (A_impl_A Γ φ H0)). simpl in H4.
+      unshelve epose proof forall_functional_subst (φ^{{evar:e↦0}}) ψ Γ H ltac:(rewrite <- mu_free_evar_quantify; exact H1) H2 ltac:(wf_auto2) ltac:(wf_auto2).
+      rewrite bevar_subst_evar_quantify in H5. wf_auto2.
+      do 2 mlIntro. mlApplyMeta H5. mlSplitAnd.
+      mlApplyMeta H4. all: mlAssumption.
+    Defined.
+
+    Goal forall (x y : TermPattern) (e : evar), TermPattern.
+    Proof.
+      intros [[x wfx mfx] fpx] [[y wfy mfy] fpy] e.
+      unshelve esplit.
+      unshelve esplit.
+      exact (x^[[evar:e↦y]]).
+      apply well_formed_free_evar_subst; assumption.
+      apply mu_free_free_evar_subst; assumption.
+      simpl in *.
+      intros. specialize (fpx Γ). specialize (fpy Γ).
+      assert (theory ⊆ Γ) by admit.
+      unfold is_functional in *.
+
+      Search patt_exists.
+      Print instantiate.
+      (* exists_functional_subst_meta *)
+      (* Ex_quan *)
+      (* congruence_ex *)
+
+      toMLGoal. wf_auto2.
+      mlAdd fpx. mlDestructEx "0" as a.
+      mlAdd fpy. mlDestructEx "1" as b.
+      mlSimpl. unfold evar_open. simpl.
+      rewrite ! bevar_subst_not_occur; only 1,2: wf_auto2.
+
+      clear fpx fpy.
+      induction x.
+      - destruct (decide (e = x)) as [-> |].
+        mlExists b. unfold evar_open. mlSimpl. simpl.
+        rewrite decide_eq_same bevar_subst_not_occur. wf_auto2.
+        mlAssumption.
+        mlExists a. unfold evar_open. mlSimpl. simpl.
+        rewrite decide_False. assumption.
+        rewrite bevar_subst_not_occur. wf_auto2.
+        mlAssumption.
+      - mlExists a. unfold evar_open. mlSimpl. simpl.
+        mlAssumption.
+      - cbn in wfx. wf_auto2.
+      - cbn in wfx. wf_auto2.
+      - mlExists a. unfold evar_open. mlSimpl. simpl.
+        mlAssumption.
+      -
+
+      destruct (decide (a = e)) as [-> |].
+      mlExists b.
+      mlSimpl. unfold evar_open. simpl.
+      rewrite ! bevar_subst_not_occur. wf_auto2.
+      mlSymmetry in "1".
+      mlRewriteBy "1" at 1.
+      replace y with ((patt_free_evar e)^[[evar:e↦y]]) at 3.
+      2: simpl; rewrite decide_eq_same; reflexivity.
+      (* Search free_evar_subst. *)
+
+      replace (x^[[evar:e↦y]] =ml (patt_free_evar e)^[[evar:e↦y]]) with ((x =ml (patt_free_evar e))^[[evar:e↦y]]) by reflexivity.
+      rewrite <- bevar_subst_evar_quantify with (dbi := 0).
+      mlApplyMeta forall_functional_subst.
+      mlSplitAnd. 2: mlExists b; mlSimpl; cbn; unfold evar_open; rewrite bevar_subst_not_occur; [wf_auto2 | mlSymmetry; mlAssumption].
+      mlClear "1". mlRevert "0". fromMLGoal.
+      epose proof universal_generalization_iter Γ [x =ml patt_free_evar e] (x =ml patt_free_evar e) e AnyReasoning ltac:(wf_auto2) ltac:(wf_auto2) ltac2:(fm_solve()) (pile_any _). cbn [foldr] in H0.
+      apply H0. aapply A_impl_A.
+      1-6: auto; try solve [wf_auto2].
+      1-3: mlSimpl; cbn; rewrite ? decide_eq_same; mlSimpl; wf_auto2; rewrite <- mu_free_evar_quantify; assumption.
+
+      Search [is_functional | patt_exists patt_equal b0].
+
+      mlExists a. mlSimpl. unfold evar_open. simpl.
+      rewrite bevar_subst_not_occur. wf_auto2.
+      replace (patt_free_evar a) with ((patt_free_evar a)^[[evar:e↦y]]) at 2.
+      2: simpl; rewrite decide_False; auto.
+      replace (x^[[evar:e↦y]] =ml (patt_free_evar a)^[[evar:e↦y]]) with ((x =ml (patt_free_evar a))^[[evar:e↦y]]) by reflexivity.
+      rewrite <- bevar_subst_evar_quantify with (dbi := 0). 2: wf_auto2.
+      mlApplyMeta forall_functional_subst.
+      mlSplitAnd.
+      2: mlExists b; mlSimpl; cbn; unfold evar_open; rewrite bevar_subst_not_occur; [wf_auto2 | mlAssumption].
+      epose proof universal_generalization_iter Γ [x =ml patt_free_evar a] (x =ml patt_free_evar a) e AnyReasoning ltac:(wf_auto2) ltac:(wf_auto2).
+
+      (**)
+
+
+
+
+      mlExists a. mlSimpl. unfold evar_open. simpl.
+      rewrite bevar_subst_not_occur. wf_auto2.
+      mlFreshEvar as q.
+      assert (e ≠ q) by ltac2:(fm_solve()).
+      unshelve epose proof equality_elimination_basic _ x (patt_free_evar a) {| pcEvar := q; pcPattern := (patt_free_evar q)^[[evar:e↦y]] =ml patt_free_evar a |} H _ _ _ _.
+      3,4: simpl; rewrite ! (decide_False _ _ H0).
+      1-4: wf_auto2.
+      simpl in H1. rewrite ! (decide_False _ _ H0) in H1.
+      unfold emplace in H1. cbn [pcPattern pcEvar] in H1.
+
+
+    mlRewriteBy "0" at 1.
+    mlSymmetry in "0".
+    mlRewriteBy "0" at 1.
+    rewrite free_evar_subst_no_occurrence.
+    ltac2:(fm_solve()).
+
+  #[refine] Instance optionSetUP `{H : ElemOf (TermPattern * TermPattern) T, H0 : Empty T, H1 : Singleton (TermPattern * TermPattern) T, H2 : Union T, H3 : Intersection T, H4 : Difference T, H5 : Elements (TermPattern * TermPattern) T, @FinSet (TermPattern * TermPattern) T H H0 H1 H2 H3 H4 H5 (@prod_eq_dec _ TermPattern_eq_dec _ TermPattern_eq_dec), !LeibnizEquiv T} : UP (option T) := {
     insertUP t x := option_map ({[x]} ∪.) t;
     bottomUP := None;
-    toPredicateUP := from_option (set_fold (WFPatt_and ∘ (fun '(x, y) => x wf=ml y)) (Top ↾ well_formed_top)) (patt_bott ↾ well_formed_bott);
-    substituteAllUP e p := option_map (set_map (fun '(x, y) => (x^wf[[evar:e↦p]], y^wf[[evar:e↦p]])));
+    toPredicateUP := from_option (set_fold (WFMF_and ∘ (fun '(x, y) => tpPattern x wf=ml tpPattern y)) wfmfTop) (mkWFMF patt_bott well_formed_bott eq_refl);
+    substituteAllUP e p := option_map (set_map (fun '(x, y) => ((tpPattern x)^wf[[evar:e↦p]], (tpPattern y)^wf[[evar:e↦p]])));
     singletonUP t1 t2 := Some {[(t1, t2)]}
   }.
   Proof.
     * intros. destruct_with_eqn t; simpl.
-      ** match goal with [ |- context[set_fold (WFPatt_and ∘ ?f') ?b' _] ] => remember f' as f; remember b' as b end.
+      ** remember (λ '(x0, y0), x0 wf=ml y0) as f.
          epose proof (elem_of_dec_slow (x, y) t0) as [].
-         pose proof (in_set_implies_in_predicate Γ f b _ _ e).
+         pose proof (in_set_implies_in_predicate Γ f wfmfTop _ _ e).
          rewrite subseteq_union_1_L. set_solver.
-         unfold WFDerives in H7 |- *. toMLGoal. apply wfWFPattern.
-         rewrite ! unwrap_wfwrapper in H7 |- *.
+         toMLGoal. apply wfmfWF.
+         rewrite ! unwrap_wfmfbWrapper in H7 |- *. simpl in H7 |- *.
          mlSplitAnd; mlDecomposeAll.
-         mlSplitAnd. subst f. rewrite unwrap_wfwrapper in H7.
+         mlSplitAnd. subst f.
+         rewrite unwrap_wfmfbWrapper in H7. simpl in H7.
          mlApplyMeta H7. 1-3: mlAssumption.
          rewrite union_comm_L.
-         opose proof* (set_fold_disj_union_strong_equiv Γ (WFPatt_and ∘ f) b t0 {[(x, y)]} _ _).
+         opose proof* (set_fold_disj_union_strong_equiv Γ (WFMF_and ∘ f) wfmfTop t0 {[(x, y)]} _ _).
          intros. subst f. simpl. do ! case_match.
-         unfold WFDerives. toMLGoal. apply wfWFPattern. rewrite ! unwrap_wfwrapper.
+         toMLGoal. apply wfmfWF. rewrite ! unwrap_wfmfbWrapper. simpl.
          mlSplitAnd; mlDecomposeAll; repeat mlSplitAnd; mlAssumption.
          set_solver.
          rewrite set_fold_singleton in H7. simpl in H7. subst f.
          exact H7.
-      ** unfold WFDerives. case_match. simpl.
-         apply (f_equal proj1_sig) in H7. rewrite ! unwrap_wfwrapper in H7. simpl in H7.
-         rewrite <- H7. toMLGoal. refine_wf; apply wfWFPattern.
+      ** case_match. simpl.
+         apply (f_equal TacticsNotations.wfmfPattern) in H7. rewrite ! unwrap_wfmfbWrapper in H7. simpl in H7.
+         rewrite <- H7. toMLGoal. refine_wf; apply TacticsNotations.wfmfWF.
          mlSplitAnd; mlDecomposeAll; mlDestructBotDocVer.
     * intros. destruct_with_eqn t; simpl.
-      ** match goal with [ |- context[set_fold (WFPatt_and ∘ ?f') ?b' (set_map ?g' _)] ] => remember f' as f; remember b' as b; remember g' as g end.
-         apply (set_fold_ind' (fun r X => Γ ⊢wf set_fold (WFPatt_and ∘ f) b (set_map g X) wf<---> r^wf[[evar:e↦p]]) (WFPatt_and ∘ f) b).
-         rewrite -> set_map_empty, set_fold_empty. subst b.
-         unfold WFDerives. rewrite ! unwrap_wfwrapper. simpl.
-         toMLGoal. wf_auto2. mlSplitAnd; mlDecomposeAll.
+      ** remember (λ '(x, y), x wf=ml y) as f.
+         remember (λ '(x, y), (x^wf[[evar:e↦p]], y^wf[[evar:e↦p]])) as g.
+         apply (set_fold_ind' (fun r X => Γ ⊢ set_fold (WFMF_and ∘ f) wfmfTop (set_map g X) wf<---> r^wf[[evar:e↦p]]) (WFMF_and ∘ f) wfmfTop).
+         rewrite -> set_map_empty, set_fold_empty.
+         toMLGoal. apply wfmfWF.
+         rewrite ! unwrap_wfmfbWrapper. simpl.
+         mlSplitAnd; mlDecomposeAll.
          mlAssumption. pose proof (top_holds Γ). use AnyReasoning in H7. mlExactMeta H7.
          intros. simpl. rewrite -> set_map_union_L, set_map_singleton_L.
          unshelve epose proof (elem_of_dec_slow (g x) (set_map g X)) as [].
-         1: exact T. 4: exact H6. 1-3: auto.
+         1: exact T.
+         exact (@prod_eq_dec _ WFMFPattern_eq_dec _ WFMFPattern_eq_dec).
+         4: exact H6. 1-3: auto.
          rewrite subseteq_union_1_L. apply elem_of_subseteq_singleton. exact e0.
-         epose proof (in_set_implies_in_predicate Γ f b _ _ e0).
-         unfold WFDerives in H8, H9 |- *. toMLGoal. apply wfWFPattern.
-         rewrite ! unwrap_wfwrapper in H8, H9 |- *.
-         cbn [flip] in H8 |- *. mlSimpl.
+         epose proof (in_set_implies_in_predicate Γ f wfmfTop _ _ e0).
+         toMLGoal. apply wfmfWF.
+         rewrite ! unwrap_wfmfbWrapper in H8, H9 |- *.
+         cbn -[patt_and] in H8, H9 |- *. mlSimpl.
          mlSplitAnd; mlDecomposeAll. mlSplitAnd.
          mlApplyMeta H9 in "0". subst f g. case_match.
-         rewrite ! unwrap_wfwrapper. cbn [flip]. mlSimpl.
+         rewrite ! unwrap_wfmfbWrapper. cbn -[patt_equal]. mlSimpl.
          mlAssumption.
          apply pf_iff_proj1 in H8. mlApplyMeta H8. mlAssumption.
-         1-2: refine_wf; apply wfWFPattern.
+         1-2: refine_wf; apply wfmfWF.
          apply pf_iff_proj2 in H8. mlApplyMeta H8. mlAssumption.
-         1-2: refine_wf; apply wfWFPattern.
+         1-2: refine_wf; apply wfmfWF.
          rewrite union_comm_L.
-         unshelve opose proof* (set_fold_disj_union_strong_equiv Γ (WFPatt_and ∘ f) b (set_map g X) {[g x]}).
+         unshelve opose proof* (set_fold_disj_union_strong_equiv Γ (WFMF_and ∘ f) wfmfTop (set_map g X) {[g x]}).
          5: exact H6. all: auto.
          intros.
          subst f g. simpl. repeat case_match.
-         unfold WFDerives. toMLGoal. apply wfWFPattern.
-         rewrite ! unwrap_wfwrapper. mlSplitAnd; mlDecomposeAll;
+         toMLGoal. apply wfmfWF.
+         rewrite ! unwrap_wfmfbWrapper. simpl. mlSplitAnd; mlDecomposeAll;
          repeat mlSplitAnd; mlAssumption.
          set_solver.
-         unfold WFDerives in H9, H8 |- *.
-         rewrite ! unwrap_wfwrapper in H9, H8 |- *.
-         cbn [flip] in H8 |- *.
+         rewrite ! unwrap_wfmfbWrapper in H8, H9 |- *.
+         cbn -[patt_and] in H8, H9 |- *.
          eapply pf_iff_equiv_trans. 4: exact H9.
-         1-3: refine_wf; apply wfWFPattern.
+         1-3: refine_wf; apply wfmfWF.
          rewrite set_fold_singleton. cbn [compose].
-         mlSimpl. rewrite unwrap_wfwrapper.
-         toMLGoal. refine_wf; apply wfWFPattern.
+         mlSimpl. rewrite unwrap_wfmfbWrapper. simpl.
+         toMLGoal. refine_wf; apply wfmfWF.
          mlSplitAnd; mlDecomposeAll; mlSplitAnd.
-         subst f g. case_match. rewrite ! unwrap_wfwrapper.
-         cbn [flip]. mlSimpl. mlAssumption.
+         subst f g. case_match. rewrite ! unwrap_wfmfbWrapper.
+         cbn -[patt_equal]. mlSimpl. mlAssumption.
          apply pf_iff_proj1 in H8. mlApplyMeta H8. mlAssumption.
-         1-2: refine_wf; apply wfWFPattern.
-         subst f g. case_match. rewrite ! unwrap_wfwrapper.
-         cbn [flip]. mlSimpl. mlAssumption.
+         1-2: refine_wf; apply wfmfWF.
+         subst f g. case_match. rewrite ! unwrap_wfmfbWrapper.
+         cbn -[patt_equal]. mlSimpl. mlAssumption.
          apply pf_iff_proj2 in H8. mlApplyMeta H8. mlAssumption.
-         1-2: refine_wf; apply wfWFPattern.
-      ** case_match. apply (f_equal proj1_sig) in H7. rewrite unwrap_wfwrapper in H7. simpl in H7. unfold WFDerives. simpl. rewrite H7. now aapply pf_iff_equiv_refl.
+         1-2: refine_wf; apply wfmfWF.
+      ** case_match. apply (f_equal TacticsNotations.wfmfPattern) in H7. rewrite unwrap_wfmfbWrapper in H7. simpl in H7. simpl. rewrite H7. now aapply pf_iff_equiv_refl.
     * intros. destruct_with_eqn t. simpl. discriminate. now destruct H7.
     * intros. simpl. rewrite set_fold_singleton. simpl.
-      unfold WFDerives. rewrite ! unwrap_wfwrapper. simpl.
-      toMLGoal. refine_wf; apply wfWFPattern.
+      rewrite ! unwrap_wfmfbWrapper. simpl.
+      toMLGoal. refine_wf; apply wfmfWF.
       mlSplitAnd; mlDecomposeAll; only 2: mlSplitAnd; try mlAssumption.
       pose proof (top_holds Γ). use AnyReasoning in H7.
       mlExactMeta H7.
@@ -194,26 +462,25 @@ Inductive unification_step {Σ : Signature} {syntax : Syntax} {T : Set} {UPT : U
       insertUP P (f wf⋅ t, g wf⋅ u) ===> insertUP (insertUP P (f, g)) (t, u)
   | symbol_clash_lUS : forall P f t,
       P ≠ bottomUP ->
-      patt_sym f ≠ `t ->
-      (forall x, `t ≠ patt_free_evar x) ->
-      insertUP P (patt_sym f ↾ well_formed_sym f, t) ===> bottomUP
+      patt_sym f ≠ wfmfPattern t ->
+      (forall x, wfmfPattern t ≠ patt_free_evar x) ->
+      insertUP P (mkWFMF (patt_sym f) (well_formed_sym f) eq_refl, t) ===> bottomUP
   | symbol_clash_rUS : forall P f t,
       P ≠ bottomUP ->
-      patt_sym f ≠ `t ->
-      (forall x, `t ≠ patt_free_evar x) ->
-      insertUP P (t, patt_sym f ↾ well_formed_sym f) ===> bottomUP
+      patt_sym f ≠ wfmfPattern t ->
+      (forall x, wfmfPattern t ≠ patt_free_evar x) ->
+      insertUP P (t, mkWFMF (patt_sym f) (well_formed_sym f) eq_refl) ===> bottomUP
   | orientUS : forall P x y,
       P ≠ bottomUP ->
-      insertUP P (x, patt_free_evar y ↾ well_formed_free_evar y) ===> insertUP P (patt_free_evar y ↾ well_formed_free_evar y, x)
+      insertUP P (x, mkWFMF (patt_free_evar y) (well_formed_free_evar y) eq_refl) ===> insertUP P (mkWFMF (patt_free_evar y) (well_formed_free_evar y) eq_refl, x)
   | occours_checkUS : forall P x t,
       P ≠ bottomUP ->
-      x ∈ free_evars (`t) ->
-      insertUP P (patt_free_evar x ↾ well_formed_free_evar x, t) ===> bottomUP
+      x ∈ free_evars (wfmfPattern t) ->
+      insertUP P (mkWFMF (patt_free_evar x) (well_formed_free_evar x) eq_refl, t) ===> bottomUP
   | eliminationUS : forall P x t,
       P ≠ bottomUP ->
-      x ∉ free_evars (`t) ->
-      mu_free (`t) ->
-      insertUP P (patt_free_evar x ↾ well_formed_free_evar x, t) ===> insertUP (substituteAllUP x t P) (patt_free_evar x ↾ well_formed_free_evar x, t)
+      x ∉ free_evars (wfmfPattern t) ->
+      insertUP P (mkWFMF (patt_free_evar x) (well_formed_free_evar x) eq_refl, t) ===> insertUP (substituteAllUP x t P) (mkWFMF (patt_free_evar x) (well_formed_free_evar x) eq_refl, t)
       where "P ===> P'" := (unification_step P P').
 
 Inductive USrtc {Σ : Signature} {syntax : Syntax} {T : Set} {UPT : UP T} : T -> T -> Set :=
