matching-logic/src/Experimental/Unification/TacticsNotations.v
@@ -9,6 +9,89 @@ Close Scope equations_scope. (* Because of [!] *)
 Section TacticsNotations.
   Context {Σ : Signature} {syntax : Syntax}.
 
+  Record WFMFPattern := mkWFMF {
+    wfmfPattern :> Pattern;
+    wfmfWF : well_formed wfmfPattern;
+    wfmfMF : mu_free wfmfPattern;
+  }.
+
+  Record TermPattern := mkTP {
+    tpPattern :> WFMFPattern;
+    tpFP : forall Γ, Γ ⊢ is_functional tpPattern;
+  }.
+
+  Record WFMFBinary := mkWFMFB {
+    wfmfbF : Pattern -> Pattern -> Pattern;
+    wfmfbWF : ∀ φ1 φ2, well_formed φ1 -> well_formed φ2 -> well_formed (wfmfbF φ1 φ2);
+    wfmfbMF : ∀ φ1 φ2, mu_free φ1 -> mu_free φ2 -> mu_free (wfmfbF φ1 φ2);
+    wfmfbWrapper :> WFMFPattern -> WFMFPattern -> WFMFPattern :=
+      λ '(mkWFMF a wfa mfa) '(mkWFMF b wfb mfb), mkWFMF
+        (wfmfbF a b)
+        (wfmfbWF a b wfa wfb)
+        (wfmfbMF a b mfa mfb)
+    ;
+  }.
+
+  Lemma unwrap_wfmfbWrapper f a b : wfmfPattern (wfmfbWrapper f a b) = wfmfbF f (wfmfPattern a) (wfmfPattern b).
+  Proof.
+    destruct f, a, b. reflexivity.
+  Defined.
+
+  (**
+     Low-level mu-free solver to avoid huge proof terms later on.
+   *)
+  Tactic Notation "solve_mf" :=
+    simpl; unfold is_true; intros;
+    repeat match goal with
+           | [ |- _ && true = true ] => refine (eq_trans (andb_true_r _) _)
+           | [ |- _ && _ = true ] => refine (andb_true_intro (conj _ _))
+           | [ mf : mu_free ?φ = true |- mu_free ?φ = true ] => exact mf
+           end.
+
+  Definition WFMF_imp := mkWFMFB
+    patt_imp
+    well_formed_imp
+    ltac:(solve_mf)
+  .
+
+  Definition WFMF_and := mkWFMFB
+    patt_and
+    well_formed_and
+    ltac:(solve_mf)
+  .
+
+  Definition WFMF_iff := mkWFMFB
+    patt_iff
+    well_formed_iff
+    ltac:(solve_mf)
+  .
+
+  Definition WFMF_equal := mkWFMFB
+    patt_equal
+    well_formed_equal
+    ltac:(solve_mf)
+  .
+
+  Definition WFMF_app := mkWFMFB
+    patt_app
+    well_formed_app
+    ltac:(solve_mf)
+  .
+
+  Definition WFMF_fevar_subst x := mkWFMFB
+    (free_evar_subst ^~ x)
+    (λ a b, well_formed_free_evar_subst x b a)
+    (λ a b H H', mu_free_free_evar_subst b a x H' H)
+  .
+  
+  (**
+     With the coercions, it should be a lot easier to write things like
+     this. WFDerives probably won't even be needed.
+   *)
+  Check λ (x y : TermPattern), WFMF_and x y.
+  Check λ (x : TermPattern) (y : WFMFPattern) Γ, Γ ⊢ WFMF_and x y.
+
+  (*
   Definition WFPattern := sig well_formed.
   Definition mkWFWrapper (f : Pattern -> Pattern -> Pattern) (wfp : forall a b, well_formed a -> well_formed b -> well_formed (f a b)) : WFPattern -> WFPattern -> WFPattern.
   Proof.
@@ -22,11 +105,41 @@ Section TacticsNotations.
   Definition WFFree_evar_subst (x : evar) := mkWFWrapper (flip free_evar_subst x) (fun a b => well_formed_free_evar_subst x b a).
   Definition WFDerives (Γ : Theory) (p : WFPattern) : Set := derives Γ (proj1_sig p).
   Definition WFPatt_app := mkWFWrapper patt_app well_formed_app.
+   *)
   Lemma well_formed_free_evar : forall e, well_formed (patt_free_evar e).
   Proof.
     exact (const eq_refl).
   Defined.
 
+  Instance WFMFPattern_eq_dec : EqDecision WFMFPattern.
+  Proof.
+    unfold EqDecision, Decision.
+    intros [φ1 wf1 mf1] [φ2 wf2 mf2].
+    destruct (decide (φ1 = φ2)) as [-> |]; [left | right; congruence].
+    rewrite (Classical_Prop.EqdepTheory.UIP _ _ _ wf1 wf2)
+            (Classical_Prop.EqdepTheory.UIP _ _ _ mf1 mf2).
+    reflexivity.
+  Defined.
+
+  Instance TermPattern_eq_dec : EqDecision TermPattern.
+  Proof.
+    unfold EqDecision, Decision.
+    intros [wfmf1 fp1] [wfmf2 fp2].
+    destruct (decide (wfmf1 = wfmf2)) as [-> |]; [left | right; congruence].
+    f_equal.
+    apply functional_extensionality_dep_good. intros Γ.
+    (**
+       There are two options here:
+       1. These proofs should be irrelevant, which they would be if our
+          proof system was in Prop.
+       2. The differences in the proofs matter, and they should be
+          compared like the patterns.
+       I don't know which is the right move here, but I found no way to
+       do either.
+     *)
+  Admitted.
+
+  (*
   Lemma lift_derives : forall Γ p, derives Γ (proj1_sig p) -> WFDerives Γ p.
   Proof.
     intros. auto.
@@ -49,16 +162,17 @@ Section TacticsNotations.
     1, 3: intros; apply eq_pi; apply decide_rel; apply bool_eq_dec.
     1, 2: apply Pattern_eqdec.
   Defined.
+   *)
 
 End TacticsNotations.
 
-Notation "a wf---> b"  := (WFPatt_imp a b) (at level 75, right associativity) : ml_scope.
-Notation "a 'wfand' b" := (WFPatt_and   a b) (at level 72, left associativity) : ml_scope.
-Notation "a wf<---> b" := (WFPatt_iff a b) (at level 74, no associativity) : ml_scope.
-Notation "p wf=ml q" := (WFPatt_equal p q) (at level 67) : ml_scope.
-Notation "e ^wf[[ 'evar:' x ↦ e' ]]" := (WFFree_evar_subst x e' e) (at level 2, e' at level 200, left associativity, format "e ^wf[[ 'evar:' x ↦ e' ]]" ) : ml_scope.
-Notation "Γ ⊢wf ϕ" := (WFDerives Γ ϕ) (at level 95, no associativity).
-Notation "a wf⋅ b" := (WFPatt_app a b) (at level 66, left associativity) : ml_scope.
+Notation "a wf---> b"  := (WFMF_imp a b) (at level 75, right associativity) : ml_scope.
+Notation "a 'wfand' b" := (WFMF_and   a b) (at level 72, left associativity) : ml_scope.
+Notation "a wf<---> b" := (WFMF_iff a b) (at level 74, no associativity) : ml_scope.
+Notation "p wf=ml q" := (WFMF_equal p q) (at level 67) : ml_scope.
+Notation "e ^wf[[ 'evar:' x ↦ e' ]]" := (WFMF_fevar_subst x e' e) (at level 2, e' at level 200, left associativity, format "e ^wf[[ 'evar:' x ↦ e' ]]" ) : ml_scope.
+(* Notation "Γ ⊢wf ϕ" := (WFDerives Γ ϕ) (at level 95, no associativity). *)
+Notation "a wf⋅ b" := (WFMF_app a b) (at level 66, left associativity) : ml_scope.
 
 Tactic Notation "mlDeductHypo" constr(name) :=
   match goal with
